Core/RefinesFacts.v
@@ -5,6 +5,7 @@ From LHL.Util Require Import
 
 From LHL.Core Require Import
   Program
+  ProgramFacts
   Specs
   Traces
   TracesFacts
@@ -13,10 +14,18 @@ From LHL.Core Require Import
 From Coq Require Import
   Program.Equality
   Relations.Relation_Operators
-  Logic.PropExtensionality.
+  Logic.PropExtensionality
+  Logic.FunctionalExtensionality
+  Logic.ClassicalChoice
+  Init.Nat
+  Arith.EqNat
+  Arith.PeanoNat.
 
 From Paco Require Import
   paco.
+
+Lemma threadDecEq : @IsEqDec ThreadName eqb.
+Admitted.
 
 (* Basic Refinement Properties *)
 
@@ -32,12 +41,355 @@ Qed.
 
 (* Eutt implies refinement *)
 
+Lemma help_eq :
+  forall n,
+  Nat.eqb n n = true.
+intros.
+induction n.
+easy.
+simpl.
+easy.
+Qed.
+
+
+Lemma floatEx {A} {B C : A -> Prop} :
+  (forall x, B x -> C x) ->
+  (exists x, B x) -> (exists x, C x).
+intros.
+destruct_all.
+exists x.
+apply H.
+easy.
+Qed.
+
+Inductive euttTrace {E F} : Trace (LEvent E F) -> Trace (LEvent E F) -> Prop :=
+| EuttTraceNil :
+    euttTrace nil nil
+| EuttTraceLSilent p q :
+    euttTrace p q ->
+    euttTrace (cons (UEvent None) p) q
+| EuttTraceRSilent p q :
+    euttTrace p q ->
+    euttTrace p (cons (UEvent None) q)
+| EuttTraceUnder p q e :
+    euttTrace p q ->
+    euttTrace (cons (UEvent (Some e)) p) (cons (UEvent (Some e)) q)
+| EuttTraceOver p q e :
+    euttTrace p q ->
+    euttTrace (cons (OEvent e) p) (cons (OEvent e) q).
+
+Lemma euttTrace_app {E F} :
+  forall p1 p2 q1 q2 : Trace (LEvent E F),
+  euttTrace p1 q1 ->
+  euttTrace p2 q2 ->
+  euttTrace (app p1 p2) (app q1 q2).
+Admitted.
+
+Inductive euttThreadTrace {E F} : Trace (ThreadLEvent E F) -> Trace (ThreadLEvent E F) -> Prop :=
+| EuttTraceThreadNil :
+    euttThreadTrace nil nil
+| EuttTraceThreadLSilent i p q :
+    euttThreadTrace p q ->
+    euttThreadTrace (cons (i, UEvent None) p) q
+| EuttTraceThreadRSilent i p q :
+    euttThreadTrace p q ->
+    euttThreadTrace p (cons (i, UEvent None) q)
+| EuttTraceThreadUnder i p q e :
+    euttThreadTrace p q ->
+    euttThreadTrace (cons (i, UEvent (Some e)) p) (cons (i, UEvent (Some e)) q)
+| EuttTraceThreadOver i p q e :
+    euttThreadTrace p q ->
+    euttThreadTrace (cons (i, OEvent e) p) (cons (i, OEvent e) q).
+
+(* Lemma compEuttTrace *)
+
+Lemma help12 {E F} :
+  forall (p : Trace (ThreadLEvent E F)),
+  forall (qc : nat -> Trace (LEvent E F)),
+  (forall i, euttTrace (projPoint i eqb p) (qc i)) ->
+  exists q,
+    euttThreadTrace p q /\
+    forall i, projPoint i eqb q = qc i.
+Admitted.
+
+Lemma euttOver {E F} :
+  forall (p q : Trace (ThreadLEvent E F)),
+  euttThreadTrace p q ->
+  projOver p = projOver q.
+intros.
+induction H.
+easy.
+easy.
+easy.
+easy.
+simpl.
+f_equal.
+easy.
+Qed.
+
+Fixpoint nones {E F} n : Trace (LEvent E F) :=
+  match n with
+  | 0 => nil
+  | S n => cons (UEvent None) (nones n)
+  end.
+
+Lemma euttTrace_nones {E F} :
+  forall n m,
+  @euttTrace E F (nones n) (nones m).
+intros.
+induction n.
+induction m.
+constructor.
+constructor.
+easy.
+constructor.
+easy.
+Qed.
+
+Inductive help_view {E F} : Trace (LEvent E F) -> Prop :=
+| HelpViewNil :
+    help_view nil
+| HelpViewEvt n e p :
+    help_view p ->
+    e <> UEvent None ->
+    help_view (app (nones n) (cons e p)).
+
+Lemma get_view {E F} :
+  forall p,
+  @help_view E F p.
+Admitted.
+
+Lemma euttTS_refl {E F} :
+  forall s, @euttTS_ E F s s.
+intros.
+destruct s.
+constructor.
+constructor.
+apply Reflexive_eutt_ieq.
+constructor.
+intros.
+apply Reflexive_eutt_ieq.
+Qed.
+
+Lemma state_finite {E F} {impl impl' : Impl E F} :
+  forall s s' t n,
+    ~(exists A (m : F A) p, t = Cont m (NoOp p)) ->
+    euttTS_ s s' ->
+    Steps (ThreadStep impl) s (nones n) t ->
+    exists n', Steps (ThreadStep impl') s' (nones n') t.
+Admitted.
+
 Theorem eutt_layerRefines {E F} : 
   forall (spec : Spec E) (impl impl' : Impl E F), 
-  euttImpl ieq impl impl' -> 
+  euttImpl impl impl' -> 
   layerRefines (spec :> impl) (spec :> impl').
 unfold euttImpl, layerRefines, specRefines, Incl, IsTraceOfSpec, Steps.
-Admitted.
+intros.
+destruct_all.
+destruct x.
+repeat rewrite projInterSteps in *.
+destruct_all.
+subst.
+simpl .
+unfold InterSteps, InterStep in *.
+simpl in *.
+unfold InterState in *.
+repeat rewrite decompSplitSteps in *.
+simpl in *.
+destruct_all.
+cut (
+  forall i, exists q : Trace (LEvent E F),
+    euttTrace (projPoint i eqb x) q /\
+    exists stf,
+      Steps (ThreadStep impl') (allIdle i) q stf
+).
+intros.
+{
+  apply choice in H2.
+  destruct_all.
+  assert (forall i, euttTrace (projPoint i eqb x) (x0 i)).
+  intros.
+  specialize (H2 i).
+  easy.
+  assert (
+    forall i, exists stf,
+      Steps (ThreadStep impl') (allIdle i) (x0 i) stf
+  ).
+  intros.
+  specialize (H2 i).
+  easy.
+  clear H2.
+  apply choice in H4.
+  destruct_all.
+  apply help12 in H3.
+  destruct_all.
+  assert (
+    forall i,
+      Steps (ThreadStep impl') (allIdle i) (projPoint i eqb x2) (x1 i)
+  ).
+  intros.
+  specialize (H4 i).
+  specialize (H2 i).
+  rewrite <- H4 in H2.
+  easy.
+  clear H2.
+  rewrite <- (decompPointSteps eqb (ThreadStep impl')) in H5.
+  2: exact threadDecEq.
+  eexists (x1, s), x2.
+  repeat split.
+  apply euttOver.
+  easy.
+  easy.
+  {
+    simpl in *.
+    clear H5 x1 H4 x0 H0.
+    generalize dependent (Init spec).
+    induction H3.
+    easy.
+    intros.
+    dependent destruction H1.
+    unfold StateStep in H0.
+    simpl in *.
+    subst.
+    apply IHeuttThreadTrace.
+    easy.
+    intros.
+    econstructor.
+    unfold StateStep.
+    easy.
+    apply IHeuttThreadTrace.
+    easy.
+    intros.
+    dependent destruction H1.
+    econstructor.
+    exact H0.
+    apply IHeuttThreadTrace.
+    easy.
+    intros.
+    dependent destruction H1.
+    unfold StateStep in H0.
+    simpl in *.
+    subst.
+    econstructor.
+    unfold StateStep.
+    easy.
+    apply IHeuttThreadTrace.
+    easy.
+  }
+}
+clear H1.
+rewrite (decompPointSteps eqb (ThreadStep impl)) in H0.
+2: exact threadDecEq.
+intros.
+specialize (H0 i).
+revert H0.
+cut (
+  forall p s s',
+    euttTS_ s s' ->
+    Steps (ThreadStep impl) s p (t i) ->
+    exists q,
+      euttTrace p q /\
+      exists stf,
+        Steps (ThreadStep impl') s' q stf
+).
+{
+  intros.
+  apply H0 with (s:=Idle).
+  constructor.
+  easy.
+}
+generalize dependent (t i).
+clear s x t i.
+intros t p.
+assert (help_view p) by apply get_view.
+induction H0.
+repeat econstructor.
+intros.
+rewrite <- Steps_app in H3.
+destruct_all.
+dependent destruction H4.
+move H3 after st''.
+assert (
+  exists st''',
+    euttTS_ st'' st''' /\
+    ThreadStep impl' x e st'''
+).
+{
+  clear H5 H3 IHhelp_view.
+  destruct e, ev.
+  2: congruence.
+  exists st''.
+  split.
+  apply euttTS_refl.
+  easy.
+  unfold ThreadStep in *.
+  dependent destruction H4.
+  exists (Cont m (impl' _ m)).
+  split.
+  constructor.
+  apply H.
+  constructor.
+  easy.
+  easy.
+  exists st''.
+  split.
+  apply euttTS_refl.
+  unfold ThreadStep in *.
+  dependent destruction H4.
+  constructor.
+  easy.
+  easy.
+}
+destruct_all.
+apply IHhelp_view with (s':=x0) in H5.
+destruct_all.
+assert (
+  exists n',
+    Steps (ThreadStep impl') s' (nones n') x
+).
+{
+  eapply state_finite.
+  unfold ThreadStep in H4.
+  unfold not.
+  intros.
+  destruct e.
+  dependent destruction H4.
+  destruct_all.
+  subst.
+  discriminate.
+  destruct_all.
+  subst.
+  discriminate.
+  congruence.
+  destruct_all.
+  subst.
+  dependent destruction H4.
+  exact H2.
+  exact H3.
+}
+destruct_all.
+eexists (nones x3 ++ e :: x1)%list.
+split.
+apply euttTrace_app.
+apply euttTrace_nones.
+destruct e, ev.
+constructor.
+easy.
+congruence.
+constructor.
+easy.
+constructor.
+easy.
+exists x2.
+rewrite <- Steps_app.
+exists x.
+split.
+easy.
+econstructor.
+exact H7.
+easy.
+easy.
+Qed.
 
 (* Crucial Refinement Properties *)
 
@@ -106,8 +458,111 @@ easy.
 easy.
 Qed.
 
+Lemma help3 {A} {xs : list A} {x : A} :
+  to_bwd (app xs (cons x nil)) = Snoc (to_bwd xs) x.
+induction xs.
+easy.
+simpl.
+rewrite IHxs.
+clear IHxs.
+destruct xs; easy.
+Qed.
+
+Fixpoint projOver_bwd {E F} (p : bwd_list (ThreadLEvent E F)) : bwd_list (ThreadEvent F) :=
+  match p with
+  | Start => Start
+  | Snoc p (i, OEvent e) => Snoc (projOver_bwd p) (i, e)
+  | Snoc p _ => projOver_bwd p
+  end.
+
+Lemma full_trace {E F G} :
+  forall (p : Trace (ThreadLEvent E F)) (q : Trace (ThreadLEvent F G)),
+  projOver p = projUnderThr q ->
+  exists (r : Trace (ThreadLEvent E G)),
+    projUnder r = projUnder p /\
+    projOver r = projOver q /\
+    IsOverObjTrace r.
+Admitted.
+
+Lemma swapEx {A B} {P : A -> B -> Prop} :
+  (exists x y, P x y) ->
+  (exists y x, P x y).
+firstorder.
+Qed.
+
+Lemma takeThr {E F G} :
+  forall (p : Trace (ThreadLEvent E F)) (q : Trace (ThreadLEvent E G)),
+    projUnder p = projUnder q ->
+    projUnderThr p = projUnderThr q.
+Admitted.
+
 Theorem layerRefines_VComp_assoc {E F G} : 
   forall  (spec : Spec E) (impl : Impl E F) (impl' : Impl F G),
     layerRefines ((overObj (spec :> impl)) :> impl') ((spec :> impl) :|> impl').
 unfold layerRefines, specRefines, Incl, IsTraceOfSpec.
-Admitted.
+intros.
+destruct_all.
+repeat rewrite decompOverObj in *.
+destruct_all.
+subst.
+simpl (USpec (overObj (spec :> impl) :> impl')) in H0.
+rewrite decompOverObj in H0.
+destruct_all.
+simpl in *.
+symmetry in H.
+assert (H' := H).
+apply full_trace in H.
+destruct_all.
+apply swapEx.
+exists x2.
+move H' after H5.
+repeat (unfold InterState in *; simpl in *).
+cut (
+  exists st : ThreadsSt E G,
+    Steps (ThreadsStep (impl |> impl')) allIdle x2 st
+).
+{
+  intros.
+  destruct_all.
+  exists (x3, snd (snd x)).
+  repeat split; try easy.
+  simpl.
+  apply takeThr in H.
+  rewrite H.
+  easy.
+}
+unfold ThreadsSt.
+unfold ThreadsStep in *.
+cut (
+  exists st, forall i,
+    (fun i sti =>
+      Steps (ThreadStep (impl |> impl')) (allIdle i) (projPoint i eqb x2) sti)
+    i (st i)
+).
+{
+  intros.
+  destruct_all.
+  exists x3.
+  rewrite (decompPointSteps eqb (ThreadStep (impl |> impl'))).
+  easy.
+  exact threadDecEq.
+}
+rewrite (decompPointSteps eqb (ThreadStep impl)) in H3.
+2: exact threadDecEq.
+rewrite (decompPointSteps eqb (ThreadStep impl')) in H1.
+2: exact threadDecEq.
+apply choice.
+intros.
+{
+  specialize (H3 x3).
+  specialize (H1 x3).
+  move H6 at bottom.
+  move H4 before H2.
+  rename x1 into tL.
+  rename x0 into tH.
+  rename x2 into tF.
+  move tL after tH.
+  move H' after H.
+  move x3 after x.
+  rename x3 into i.
+}
