Core/Simulates.v
@@ -8,15 +8,13 @@ Section Sim.
           (spec : Spec E) (* concrete *)
           (spec' : Spec E) (* abstract *).
 
-  CoInductive Simulates_ (s1 : spec.(State)) (s1' : spec'.(State)) : Prop :=
+  CoInductive Simulates (s1 : spec.(State)) (s1' : spec'.(State)) : Prop :=
   | SimStep :
       (forall ev s2,
          spec.(Step) s1 ev s2 ->
-         exists2 s2',
-           spec'.(Step) s1' ev s2' &
-           Simulates_ s2 s2') ->
-      Simulates_ s1 s1'.
-
-  Definition Simulates : Prop := Simulates_ spec.(Init) spec'.(Init).
+         exists s2',
+           spec'.(Step) s1' ev s2' /\
+           Simulates s2 s2') ->
+      Simulates s1 s1'.
 
 End Sim.
