Core/SimulatesFacts.v
@@ -1,38 +1,40 @@
 From Coq Require Import 
-    List.
+  List
+  Program.Equality.
 
 From LHL.Util Require Import
-    TransUtil.
+  TransUtil
+  Tactics.
 
 From LHL.Core Require Import
-    Program
-    Specs
-    Traces
-    Simulates.
+  Program
+  Specs
+  Traces
+  Simulates.
 
 From LHL.Core Require Import
-    TracesFacts.
+  TracesFacts.
 
 Lemma simulate_isPathOf {E} {spec spec' : Spec E} : 
-    forall t s1 s1' s2,
-    Simulates_ spec spec' s1 s1' -> 
-    IsPathOf s1 t s2 (Steps spec.(Step)) -> 
-    exists s2', IsPathOf s1' t s2' (Steps spec'.(Step)).
-Proof. 
-    induction t.
-    - intros; exists s1'; constructor.
-    - intros. inversion H0. subst.
-      destruct H. apply (H a st'') in H3.
-      destruct H3. 
-      destruct (IHt st'' x s2 H2 H5).
-      exists x0. eapply StepsMore. apply H1. apply H3.
+  forall t s1 s1' s2,
+  Simulates spec spec' s1 s1' -> 
+  Steps spec.(Step) s1 t s2 -> 
+  exists s2', Steps spec'.(Step) s1' t s2'. 
+induction t.
+- intros; exists s1'; constructor.
+- intros. inversion H0. subst.
+  destruct H. apply (H a st'') in H3.
+  destruct H3. destruct H1.
+  destruct (IHt st'' x s2 H2 H5).
+  exists x0. eapply StepsMore. apply H1. apply H3.
 Qed.
 
 Theorem simulates_refines {E} :
-    forall (spec spec' : Spec E),
-        Simulates spec spec' -> 
-        specRefines spec spec'.
-Proof.
-    unfold specRefines, Incl, IsTraceOfSpec in *. intros. 
-    destruct H0; eapply simulate_isPathOf; eassumption.
-Qed.
+  forall (spec spec' : Spec E),
+  Simulates spec spec' (Init spec) (Init spec') -> 
+  specRefines spec spec'.
+unfold specRefines, Incl, IsTraceOfSpec.
+intros.
+destruct_all.
+dependent destruction H.
+Admitted.
